\section{Conditional independence in probability models}
\begin{enumerate}
\item We can write $p(x_{i})=\sum_{j}f_{j}(x_{i})\pi_{j}$ because according
to marginalization, \begin{eqnarray*}
p(x_{i}) & = & \sum_{j=1}^{k}p(x_{i},z_{i}=j)\\
 & = & \sum_{j=1}^{k}p(x_{i}|z_{i}=j)p(z_{i}=j)\\
 & = & \sum_{j}f_{j}(x_{i})\pi_{j}\end{eqnarray*}
.
\item The formula for $p(x_{1},\dots,x_{n})$ is $\prod_{i=1}^{n}\sum_{j=1}^{k}f_{j}(x_{i})\pi_{j}$
by the derivation below. \begin{align*}
p(x_{1},\dots,x_{n})= & \;\prod_{i=1}^{n}p(x_{i})\\
= & \;\prod_{i=1}^{n}\sum_{j}f_{j}(x_{i})\pi_{j}\end{align*}

\item The formula for $p(z_{u}=v\mid x_{1},\dots,x_{n})$ is $\ldots$ by
the derivation below. \begin{align*}
p(z_{u}=v\mid x_{1},\dots,x_{n})= & \;\frac{p(x_{1},\dots,x_{n}|z_{u}=v)p(z_{u}=v)}{p(x_{1},\dots,x_{n})}\\
= & \;\frac{p(x_{1}|z_{u}=v)...p(x_{u}|z_{u}=v)...p(x_{n}|z_{u}=v)p(z_{u}=v)}{p(x_{1},\dots,x_{n})}\\
= & \;\frac{(\prod_{i\neq u}p(x_{i}))*f_{v}(x_{u})\pi_{v}}{\prod_{i=1}^{n}p(x_{i})}\\
= & \;\frac{f(x_{u})\pi_{v}}{p(x_{u})}\\
= & \;\frac{f(x_{u})\pi_{v}}{\sum_{j=1}^{k}f_{j}(x_{u})\pi_{j}}\end{align*}
 
\end{enumerate}
