\section{Conditional independence in probability models}

\begin{enumerate} 
\item We can write $p(x_i) = \ldots$ because $\ldots$.

\item The formula for $p(x_1, \dots, x_n)$ is $\ldots$ by the
  derivation below.
  \begin{align*}
    p(x_1, \dots, x_n) =&\; \ldots \\
    =&\; \ldots
  \end{align*}

\item The formula for $p(z_u = v \mid x_1, \dots, x_n)$ is $\ldots$ by
  the derivation below.
  \begin{align*}
    p(z_u = v \mid x_1, \dots, x_n) =&\; \ldots \\
    =&\; \ldots
  \end{align*}
\end{enumerate}
